attempt to simplify FOL compiler

deps/poulet4/lib/P4automata/CompileConfRel.v
@@ -1,4 +1,5 @@
 From Equations Require Import Equations.
+Require Import Coq.Program.Equality.
 Require Import Coq.Classes.EquivDec.
 Require Import Poulet4.FinType.
 Require Import Poulet4.P4automata.ConfRel.
@@ -38,13 +39,24 @@ Section CompileConfRel.
       compile_var (BVarRest y) :=
         VThere _ (compile_bctx _) _ (Bits (check_bvar y)) (compile_var y) }.
 
+  Definition compile_bval {c: bctx} (v: bval c) : valu _ (fm_model a) (compile_bctx c).
+  Admitted.
+
+  Definition decompile_val {c: bctx} (v: valu _ (fm_model a) (compile_bctx c)) : bval c.
+  Admitted.
+
+  Lemma bval_roundtrip:
+    forall {c: bctx} (valu: _ (fm_model a) (compile_bctx c)),
+      compile_bval (decompile_val valu) = valu.
+  Proof.
+  Admitted.
+
   Equations compile_bit_expr
             {c: bctx}
-            {c': ctx (sig a)}
             (b1 b2: nat)
-            (q: tm (sig a) (app_ctx c' (compile_bctx c)) (ConfigPair b1 b2))
+            (q: tm (sig a) (compile_bctx c) (ConfigPair b1 b2))
             (e: bit_expr H c)
-    : tm (sig a) (app_ctx c' (compile_bctx c)) (be_sort b1 b2 e) :=
+    : tm (sig a) (compile_bctx c) (be_sort b1 b2 e) :=
     { compile_bit_expr q (BELit _ _ l) :=
         TFun (sig a) (BitsLit a (List.length l) (l2t l)) TSNil;
       compile_bit_expr q (BEBuf _ _ Left) :=
@@ -60,7 +72,7 @@ Section CompileConfRel.
         let store := TFun (sig a) (Store2 a b1 b2) (TSCons q TSNil) in
         TFun (sig a) (Lookup a (projT1 h)) (TSCons store (TSCons key TSNil));
       compile_bit_expr q (BEVar _ b) :=
-        TVar (reindex_var (compile_var b));
+        TVar (compile_var b);
       compile_bit_expr q (BESlice e hi lo) :=
         TFun (sig a) (Slice a _ hi lo) (TSCons (compile_bit_expr q e) TSNil);
       compile_bit_expr q (BEConcat e1 e2) :=
@@ -68,11 +80,10 @@ Section CompileConfRel.
 
   Equations compile_store_rel
             {c: bctx}
-            {c': ctx (sig a)}
-            (b1 b2: nat)
-            (q: tm (sig a) (app_ctx c' (compile_bctx c)) (ConfigPair b1 b2))
+            {b1 b2: nat}
+            (q: tm (sig a) (compile_bctx c) (ConfigPair b1 b2))
             (r: store_rel H c)
-            : fm (sig a) (app_ctx c' (compile_bctx c)) :=
+            : fm (sig a) (compile_bctx c) :=
     { compile_store_rel q BRTrue := FTrue;
       compile_store_rel q BRFalse := FFalse;
       compile_store_rel q (BREq e1 e2) :=
@@ -94,12 +105,13 @@ Section CompileConfRel.
               (compile_store_rel q r2)
     }.
 
+  Obligation Tactic := idtac.
+
   Definition compile_conf_rel
-    {c': ctx (sig a)}
     {n m: nat}
     (r: conf_rel S H)
-    (q: tm (sig a) c' (ConfigPair n m))
-    : fm (sig a) c'
+    (q: tm (sig a) (CEmp _) (ConfigPair n m))
+    : fm (sig a) (CEmp _)
   :=
     let s1 := r.(cr_st).(cs_st1).(st_state) in
     let s2 := r.(cr_st).(cs_st2).(st_state) in
@@ -111,27 +123,27 @@ Section CompileConfRel.
     let s2eq :=
         FEq (TFun (sig a) (State2 a n m)
                   (TSCons q TSNil))
-            (TFun (sig a) (StateLit _ s1) TSNil)
+            (TFun (sig a) (StateLit _ s2) TSNil)
     in
-    let sr := quantify _ (compile_store_rel (weaken_tm _ q) r.(cr_rel)) in
-    FImpl s1eq (FImpl s2eq sr).
+    let sr: fm (sig a) _ :=
+        (compile_store_rel (reindex_tm q) r.(cr_rel))
+    in
+    FImpl s1eq (FImpl s2eq (quantify_all _ sr)).
 
   Definition compile_crel
-    {c': ctx (sig a)}
     {n m: nat}
     (R: crel S H)
-    (i: fm (sig a) c')
-    (q: tm (sig a) c' (ConfigPair n m))
-    : fm (sig a) c' :=
+    (i: fm (sig a) (CEmp _))
+    (q: tm (sig a) (CEmp _) (ConfigPair n m))
+    : fm (sig a) (CEmp _) :=
     List.fold_right (fun r f => FAnd _ (compile_conf_rel r q) f) i R.
 
   Definition compile_entailment
-    {c': ctx (sig a)}
     {n m: nat}
     (e: entailment S H)
-    (i: fm (sig a) c')
-    (q: tm (sig a) c' (ConfigPair n m))
-    : fm (sig a) c' :=
+    (i: fm (sig a) (CEmp _))
+    (q: tm (sig a) (CEmp _) (ConfigPair n m))
+    : fm (sig a) (CEmp _) :=
     (FImpl (compile_crel e.(e_prem) i q)
            (compile_conf_rel e.(e_concl) q)).
 
@@ -146,12 +158,38 @@ Section CompileConfRel.
         exist (fun c => c.(conf_buf_len) = q2.(conf_buf_len)) q2 eq_refl in
     TFun (sig a) (ConfPairLit (q1', q2')) TSNil.
 
+  Lemma compile_store_rel_correct:
+    forall c (r: store_rel H c) valu q1 q2,
+      interp_store_rel r valu q1 q2 <->
+      interp_fm (m := fm_model a) (compile_bval valu)
+                (compile_store_rel (compile_config q1 q2) r).
+  Proof.
+  Admitted.
+
   Lemma compile_conf_rel_correct:
     forall r q1 q2,
       interp_conf_rel a r q1 q2 <->
       interp_fm (m := fm_model a) (VEmp _ _) (compile_conf_rel r (compile_config q1 q2)).
   Proof.
-  Admitted.
+    destruct r.
+    unfold interp_conf_rel, compile_conf_rel.
+    unfold interp_conf_state, interp_state_template.
+    simpl.
+    intros q1 q2.
+    repeat (progress cbn || autorewrite with interp_fm mod_fns weaken_tm).
+    autorewrite with interp_fm.
+    setoid_rewrite quantify_all_correct; eauto.
+    setoid_rewrite compile_store_rel_correct.
+    fold (compile_bctx cr_ctx).
+    intuition.
+    - specialize (H3 (eq_sym H1) (eq_sym H2)).
+      specialize (H3 (decompile_val valu)).
+      rewrite bval_roundtrip in H3.
+      auto.
+    - specialize (H0 (eq_sym H2) (eq_sym H3)).
+      specialize (H0 (compile_bval valu)).
+      apply H0.
+  Qed.
 
   Lemma compile_crel_correct:
     forall R i ifm q1 q2,
